\documentclass{book}
\usepackage{graphicx}
\usepackage{listings}
\usepackage{color}
\usepackage{graphicx}
\usepackage{booktabs}
\usepackage{fancyhdr}
\usepackage{amsmath}
\usepackage{hyperref}
\usepackage{csquotes}
\usepackage[english]{babel}
\pagestyle{fancy}
\fancyhf{}
\headheight = 0.1 in
%\rhead{\includegraphics[width=2cm, height=1cm]{logo}}
\lhead{\textbf{\Large{Problem 1 - Chain Rule Quiz}}}
\lfoot{COPYRIGHT Â©TALENTSPRINT, 2020. ALL RIGHTS RESERVED.}
\rfoot{\thepage}

\begin{document}
In the following quiz, you will practice how to use the chain rule. Some
questions look tricky, but just stick to the rules you know!
\begin{enumerate}
	\item If $f(x) = g(h(x))$, what is the differential of $f$ with respect to $x$, in terms of $g$ and $h$?
	\begin{enumerate}
		\item $f'(x) = g'(h'(x))$
		\item $f'(x) = g'(h'(x))h'(x)$
		\item $f'(x) = g'(h(x))$
		\item $f'(x) = g'(h(x))h'(x)$
	\end{enumerate}
\textbf{Answer : d} 
\\
	\item Differentiate with respect to $x$ the function
	$f(x) = \sqrt{x^3 - 2x = (x^3 - 2x)^\frac{1}{2}}$
	\begin{enumerate}
		\item $f'(x) = \frac{1}{2\sqrt{x^3 - 2x}}$
		\item $f'(x) = \frac{3x^2 - 2}{2\sqrt{x^3 - 2x}}$
		\item $f'(x) = \frac{x^3 - 2x}{2\sqrt{x^3 - 2x}}$
		\item $f'(x) = \sqrt{(3x^2 - 2)}$
	\end{enumerate}
\textbf{Answer : b} 
\\
	\item Differentiate with respect to $x$ the function $f(x) = e^{x^3-3}$
	\begin{enumerate}
		\item $f'(x) = 3x^2e^{x^3-3}$
		\item $f'(x) = e^{3x^2}$
		\item $f'(x) = (x^3-3)e^{3x^2}$
		\item $f'(x) = (x^3-3)e^{x^3-3}$
	\end{enumerate}
\textbf{Answer : a} 
\\
	\item Differentiate with respect to $x$ the function $f(x) = \sqrt{e^{x+2}}$
	\begin{enumerate}
		\item $f'(x) = \frac{\sqrt{e^{x+2}}}{2}$
		\item $f'(x) = \sqrt{e^{x+2}}$
		\item $f'(x) = \frac{1}{2e^{x+2}}$
		\item $f'(x) = \frac{1}{\sqrt{e^{x+2}}}$
	\end{enumerate}
\textbf{Answer : a} 
\\
	\item If $f{t} = f(y(x(t)))$, what is the diferential of $f$ with respect to $t$, in terms of $f$, $y$, $x$ and $t$?
	\begin{enumerate}
		\item $f'(t) = f'(y'(x'(t))).y'(x'(t)).x'(t)$
		\item $f'(t) = f'(y(x(t))).y'(x(t))$
		\item $f'(t) = f'(y'(x'(t)))$
		\item $f'(t) = f'(y(x(t))).y'(x(t)).x'(t)$
	\end{enumerate}
\textbf{Answer : d} 
\end{enumerate}
\end{document}